More substitute preserves typing lemma progress

src/Language/PlutusIR/Semantics/Dynamic/AnnotationSubstitution.v
@@ -20,11 +20,6 @@ Definition tyvars_bound_by_binding (b : NamedTerm.Binding) : list tyname :=
 Definition tyvars_bound_by_bindings (bs : list NamedTerm.Binding) : list tyname := List.concat (map tyvars_bound_by_binding bs).
 
 (** ** Implementation as an inductive datatype *)
-Definition substituteA_constructor (X : tyname) (S : Ty) (c : constructor) : constructor :=
-  match c with
-  | Constructor (VarDecl x T) ar => Constructor (VarDecl x (substituteT X S T)) ar
-  end.
-
 Inductive substituteA : tyname -> Ty -> Term -> Term -> Prop :=
   | SA_Let1 : forall X S bs t0 bs',
       In X (tyvars_bound_by_bindings bs) ->
@@ -51,9 +46,10 @@ Inductive substituteA : tyname -> Ty -> Term -> Term -> Prop :=
       X <> bX ->
       substituteA X S t0 t0' ->
       substituteA X S (TyAbs bX K t0) (TyAbs bX K t0')
-  | SA_LamAbs : forall X S bx T t0 t0',
+  | SA_LamAbs : forall X S bx T T' t0 t0',
       substituteA X S t0 t0' ->
-      substituteA X S (LamAbs bx T t0) (LamAbs bx (substituteT X S T) t0')
+      substituteTCA X S T T' ->
+      substituteA X S (LamAbs bx T t0) (LamAbs bx (beta_reduce T') t0')
   | SA_Apply : forall X S t1 t2 t1' t2',
       substituteA X S t1 t1' ->
       substituteA X S t2 t2' ->
@@ -62,14 +58,18 @@ Inductive substituteA : tyname -> Ty -> Term -> Term -> Prop :=
       substituteA X S (Constant u) (Constant u)
   | SA_Builtin : forall X S d,
       substituteA X S (Builtin d) (Builtin d)
-  | SA_TyInst : forall X S t0 T t0',
+  | SA_TyInst : forall X S t0 T t0' T',
       substituteA X S t0 t0' ->
-      substituteA X S (TyInst t0 T) (TyInst t0' (substituteT X S T))
-  | SA_Error : forall X S T,
-      substituteA X S (Error T) (Error (substituteT X S T))
-  | SA_IWrap : forall X S F T t0 t0',
+      substituteTCA X S T T' ->
+      substituteA X S (TyInst t0 T) (TyInst t0' (beta_reduce T'))
+  | SA_Error : forall X S T T',
+      substituteTCA X S T T' ->
+      substituteA X S (Error T) (Error (beta_reduce T'))
+  | SA_IWrap : forall X S F F' T T' t0 t0',
       substituteA X S t0 t0' ->
-      substituteA X S (IWrap F T t0) (IWrap (substituteT X S F) (substituteT X S T) t0')
+      substituteTCA X S F F' ->
+      substituteTCA X S T T' ->
+      substituteA X S (IWrap F T t0) (IWrap (beta_reduce F') (beta_reduce T') t0')
   | SA_Unwrap : forall X S t0 t0',
       substituteA X S t0 t0' ->
       substituteA X S (Unwrap t0) (Unwrap t0') 
@@ -96,13 +96,30 @@ with substituteA_bindings_rec : tyname -> Ty -> list Binding -> list Binding -> 
       substituteA_bindings_rec X S (b :: bs) (b' :: bs')
 
 with substituteA_binding : tyname -> Ty -> Binding -> Binding -> Prop :=
-  | SA_TermBind : forall X S strictness bx T t t',
+  | SA_TermBind : forall X S strictness bx T T' t t',
       substituteA X S t t' ->
-      substituteA_binding X S (TermBind strictness (VarDecl bx T) t) (TermBind strictness (VarDecl bx (substituteT X S T)) t')
-  | SA_TypeBind : forall X S tvd T,
-      substituteA_binding X S (TypeBind tvd T) (TypeBind tvd (substituteT X S T))
-  | SA_DatatypeBind : forall X S tvd YKs matchFunc cs,
-      substituteA_binding X S (DatatypeBind (Datatype tvd YKs matchFunc cs)) (DatatypeBind (Datatype tvd YKs matchFunc (map (substituteA_constructor X S) cs))).
+      substituteTCA X S T T' ->
+      substituteA_binding X S (TermBind strictness (VarDecl bx T) t) (TermBind strictness (VarDecl bx (beta_reduce T')) t')
+  | SA_TypeBind : forall X S tvd T T',
+      substituteTCA X S T T' ->
+      substituteA_binding X S (TypeBind tvd T) (TypeBind tvd (beta_reduce T'))
+  | SA_DatatypeBind : forall X S tvd YKs matchFunc cs cs',
+      substituteA_constructors X S cs cs' ->
+      substituteA_binding X S (DatatypeBind (Datatype tvd YKs matchFunc cs)) (DatatypeBind (Datatype tvd YKs matchFunc cs'))
+      
+with substituteA_constructors : tyname -> Ty -> list constructor -> list constructor -> Prop :=
+  | SA_NilC : forall X S,
+      substituteA_constructors X S nil nil
+  | SA_ConsC : forall X S c c' cs cs',
+      substituteA_constructor X S c c' ->
+      substituteA_constructors X S cs cs' ->
+      substituteA_constructors X S (c :: cs) (c' :: cs')
+
+with substituteA_constructor : tyname -> Ty -> constructor -> constructor -> Prop :=
+  | SA_Constr : forall X S T T' bx ar,
+      substituteTCA X S T T' ->
+      substituteA_constructor X S (Constructor (VarDecl bx T) ar) (Constructor (VarDecl bx (beta_reduce T')) ar)
+.
 
 #[export] Hint Constructors substituteA : core.
 #[export] Hint Constructors substituteA_bindings_nonrec : core.
