src/Language/PlutusIR/Semantics/TypeSafety/SubstitutionPreservesTyping/AnnotationSubstitution.v
@@ -6,89 +6,152 @@ Require Import PlutusCert.Language.PlutusIR.Semantics.TypeSafety.SubstitutionPre
 
 Require Import Coq.Logic.FunctionalExtensionality.
 
-Definition upd (a : tyname) (T' : Ty ) (Gamma : partial_map Ty) :=
-  fun x =>
-    match Gamma x with
-    | None => None
-    | Datatypes.Some T => Datatypes.Some (substituteT a T' T)
-    end.
+Definition tass := list (name * Ty).
 
-Lemma upd_empty : forall X U,
-    upd X U empty = empty.
+Fixpoint mupdate {X:Type} (m : partial_map X) (xts : list (string * X)) :=
+  match xts with
+  | nil => m
+  | ((x, v) :: xts') => x |-> v ; (mupdate m xts')
+  end.
+  
+Fixpoint lookup {X:Type} (k : string) (l : list (name * X)) : option X :=
+  match l with
+  | nil => None
+  | (j,x) :: l' => if String.eqb j k then Datatypes.Some x else lookup k l'
+  end.
+
+Fixpoint drop {X:Type} (n:string) (nxs:list (string * X)) : list (string * X) :=
+  match nxs with
+  | nil => nil
+  | (n',x) :: nxs' => if String.eqb n' n then drop n nxs' else (n',x) :: (drop n nxs')
+  end.
+
+Inductive UpdateContext (X : tyname) (U : Ty) : tass -> tass -> Prop :=
+  | UC_nil :
+      UpdateContext X U nil nil
+  | UC_Some : forall x T T' c c',
+      UpdateContext X U c c' ->
+      substituteTCA X U T T' ->
+      UpdateContext X U ((x, T) :: c) ((x, T') :: c').
+
+Lemma UpdateContext_domains_match : forall X U c c',
+    UpdateContext X U c c' ->
+    forall x T,
+      lookup x c = Datatypes.Some T ->
+      exists T',
+        lookup x c' = Datatypes.Some T'.
 Proof.
-  intros X U.
-  unfold upd.
-  simpl.
-  reflexivity.
+  intros X U c c' UC.
+  induction UC; intros x0 T0 C.
+  - discriminate.
+  - simpl. 
+    simpl in C.
+    destruct (x =? x0) eqn:Heqb.
+    + exists T'. auto.
+    + apply IHUC with T0.
+      auto.
 Qed.
 
-Lemma upd__substituteT : forall Gamma x X U T,
-    Gamma x = Datatypes.Some T ->
-    (upd X U Gamma) x = Datatypes.Some (substituteT X U T).
+Lemma UpdateContext_substituteTCA : forall X U c c',
+    UpdateContext X U c c' ->
+    forall x T T',
+      lookup x c = Datatypes.Some T ->
+      lookup x c' = Datatypes.Some T' ->
+      substituteTCA X U T T'.
 Proof.
-  intros.
-  unfold upd.
-  rewrite H.
-  reflexivity.
+  intros X U c c' UC.
+  induction UC; intros x' T0' T0'' E1 E2.
+  - destruct x'; discriminate.
+  - inversion E1. subst.
+    inversion E2. subst.
+    destruct (x =? x').
+    + inversion H1. subst.
+      inversion H2. subst.
+      assumption. 
+    + apply IHUC with x'; assumption.
 Qed.
 
-Lemma upd_absorbs_substituteT : forall x X U T Delta Gamma,
-    x |T-> (substituteT X U T); (Delta, upd X U Gamma) = (Delta, upd X U (x |-> T; Gamma)).
+Lemma mupdate_lookup : forall (c : tass) (x : name),
+    lookup x c = (mupdate empty c) x.
 Proof.
-  intros.
-  unfold extendT.
-  simpl.
-  f_equal.
-  apply functional_extensionality.
-  intros.
-  destruct (x =? x0) eqn:Heqb.
-  - (* x = x0 *)
-    apply eqb_eq in Heqb as Heq.
-    subst.
-    unfold upd.
-    rewrite update_eq.
-    rewrite update_eq.
+  induction c.
+  - intros.
+    simpl.
     reflexivity.
-  -  (* x <> x0 *)
-    apply eqb_neq in Heqb as Hneq.
-    unfold upd.
-    rewrite update_neq; auto.
-    rewrite update_neq; auto.
+  - intros.
+    simpl.
+    destruct a.
+    destruct (s =? x) eqn:Heqb.
+    + apply eqb_eq in Heqb as Heq.
+      subst.
+      rewrite update_eq.
+      reflexivity.
+    + apply eqb_neq in Heqb as Hneq.
+      rewrite update_neq; auto.
 Qed.
-
 
 (** ** Predicates *)
 Definition P_Term (t : Term) :=
-  forall Delta Gamma X K U T t',
-    (X |K-> K; (Delta, Gamma)) |-+ t : T ->
-    empty |-* U : K ->
-    substituteA X U t t' ->
-    (Delta, upd X U Gamma) |-+ t' : (substituteT X U T).
+  forall Delta Gamma Gamma' X U c c', 
+    UpdateContext X U c c' ->
+    Gamma = mupdate empty c ->
+    Gamma' = mupdate empty c' -> 
+    forall K t' T T',
+      (X |K-> K; (Delta, Gamma)) |-+ t : T ->
+      empty |-* U : K ->
+      substituteA X U t t' ->
+      substituteTCA X U T T' ->
+      (Delta, Gamma') |-+ t' : T'.
     
 Definition P_Binding (b : Binding) : Prop :=
-  forall Delta Gamma X K U b',
-    (X |K-> K; (Delta, Gamma)) |-ok b ->
-    empty |-* U : K ->
-    substituteA_binding X U b b' ->
-    (Delta, upd X U Gamma) |-ok b'.
+  forall Delta Gamma Gamma' X U c c',
+    UpdateContext X U c c' ->
+    Gamma = mupdate empty c ->
+    Gamma' = mupdate empty c' ->
+    forall K b',
+      (X |K-> K; (Delta, Gamma)) |-ok b ->
+      empty |-* U : K ->
+      substituteA_binding X U b b' ->
+      (Delta, Gamma') |-ok b'.
 
 
 Theorem substituteA_preserves_typing : 
   forall t, P_Term t.
 Proof.
   apply Term__ind with P_Binding.
-  - apply skip.
+  (*- apply skip.
   - (* Var *)
     intros x. 
     unfold P_Term. 
-    intros Delta Gamma X K U T t' Htyp Hkind Hsa__t'.
+    intros Delta Gamma X K U T t' c c' Gamma' T'. 
+    intros UC Heq Heq' Htyp Hkind Hsa__t' Hstca__T'.
+
+    assert (forall x, (mupdate empty c) x = lookup x c). {
+      intros. erewrite mupdate_lookup. auto.
+    }
 
     inversion Htyp. subst.
     inversion Hsa__t'. subst.
 
+    simpl in H2.
+    rewrite H in H2.
+
+    destruct (UpdateContext_domains_match _ _ _ _ UC _ _ H2) as [T0' Hlu__T'].
+
+    apply T_Var.
+    + simpl. rewrite <- mupdate_lookup. assumption. apply Hlu__T'. apply UpdateContext_substituteTCA.
+
+    eapply UpdateContext_domains_match in UC.
+    + apply T_Var.
+      simpl.
+        simpl in H2.
+        apply UC.
+      apply H2.
+
     apply T_Var.
     simpl in H1.
     simpl.
+    apply skip.
     apply upd__substituteT.
     assumption.
   - (* TyAbs*) 
@@ -188,7 +251,7 @@ Proof.
     inversion Htyp. subst.
     inversion Hsa__t'. subst.
 
-    assert ((Delta, upd X U Gamma) |-+ t0' : (substituteT X U (Ty_Forall X0 K2 T1))) by eauto.
+    assert ((Delta, UpdateContext X U Gamma) |-+ t0' : (substituteT X U (Ty_Forall X0 K2 T1))) by eauto.
     
     simpl in H.
     destruct (X =? X0) eqn:Heqb.
@@ -237,6 +300,6 @@ Proof.
     intros Delta Gamma X L U T t' Htyp Hkind Hsa__t'.
     
     inversion Htyp. subst.
-    inversion Hsa__t'. subst.
+    inversion Hsa__t'. subst.*)
 
 Admitted.
