src/Language/PlutusIR/Semantics/SemanticEquivalence/CompatibilityLemmas/Constant.v
@@ -33,15 +33,22 @@ Proof.
     assumption.
 Qed.
 
-Lemma msubstT_TyConstant : forall ss u,
-    msubstT ss (Ty_Builtin (Some (TypeIn u))) = Ty_Builtin (Some (TypeIn u)).
+Lemma msubstTCA_TyConstant : forall ss u T',
+    msubstTCA ss (Ty_Builtin (Some (TypeIn u))) T' ->
+    T' = Ty_Builtin (Some (TypeIn u)).
 Proof.
   induction ss.
-  - reflexivity.
   - intros.
-    simpl.
-    destruct a.
+    inversion H.
+    subst.  
+    reflexivity.
+  - intros.
+    inversion H.
+    subst.
+    inversion H2.
+    subst.
     apply IHss.
+    auto.
 Qed.
 
 Lemma compatibility_Constant : forall Delta Gamma u a,
@@ -68,8 +75,18 @@ Proof.
 
   autorewrite with RC.
 
-  split. { rewrite msubstT_TyConstant. apply T_Constant. }
-  split. { rewrite msubstT_TyConstant. apply T_Constant. }
+  split. { 
+    eexists. 
+    split.
+    - apply skip.
+    - apply T_Constant.  
+  }
+  split. { 
+    eexists. 
+    split.
+    - apply skip.
+    - apply T_Constant.  
+  }
 
   intros j Hlt__j e_f Hev__e_f.
 
