src/Language/PlutusIR/Semantics/Static/TypeSubstitution/CaptureAvoiding.v
@@ -1,0 +1,71 @@
+Require Import PlutusCert.Language.PlutusIR. 
+Import NamedTerm.
+Require Import PlutusCert.Language.PlutusIR.Semantics.Static.Theorems.ContextInvariance.AFI.
+Require Import PlutusCert.Language.PlutusIR.Semantics.Static.TypeSubstitution.
+
+Require Import Coq.Lists.List.
+Require Import Coq.Strings.String.
+Local Open Scope string_scope.
+
+(** * Capture-avoiding ubstitution of types *)
+
+(** ** Implementation as an inductive datatype *)
+Inductive substituteTCA (a : tyname) (U : Ty) : Ty -> Ty -> Prop :=
+  | STCA_TyVar1 : 
+      substituteTCA a U (Ty_Var a) U
+  | STCA_TyVar2 : forall b,
+      a <> b ->
+      substituteTCA a U (Ty_Var b) (Ty_Var b)
+  | STCA_TyFun : forall T1 T1' T2 T2',
+      substituteTCA a U T1 T1' ->
+      substituteTCA a U T2 T2' ->
+      substituteTCA a U (Ty_Fun T1 T2) (Ty_Fun T1' T2')
+  | STCA_TyIFix : forall F F' T T',
+      substituteTCA a U F F' ->
+      substituteTCA a U T T' ->
+      substituteTCA a U (Ty_IFix F T) (Ty_IFix F' T')
+  | STCA_TyForall1 : forall K T,
+      substituteTCA a U (Ty_Forall a K T) (Ty_Forall a K T)
+  | STCA_TyForall2 : forall b c K T T',
+      a <> b ->
+      appears_free_in_Ty b U ->
+      ~ appears_free_in_Ty c U ->
+      substituteTCA a U (substituteT b (Ty_Var c) T) T' ->
+      substituteTCA a U (Ty_Forall b K T) (Ty_Forall c K T')
+  | STCA_TyForall3 : forall b K T T',
+      a <> b ->
+      ~ appears_free_in_Ty b U ->
+      substituteTCA a U T T' ->
+      substituteTCA a U (Ty_Forall b K T) (Ty_Forall b K T')
+  | STCA_TyBuiltin : forall d,
+      substituteTCA a U (Ty_Builtin d) (Ty_Builtin d)
+  | STCA_TyLam1 : forall K T,
+      substituteTCA a U (Ty_Lam a K T) (Ty_Lam a K T)
+  | STCA_TyLam2 : forall b c K T T',
+      a <> b ->
+      appears_free_in_Ty b U ->
+      ~ appears_free_in_Ty c U ->
+      substituteTCA a U (substituteT b (Ty_Var c) T) T' ->
+      substituteTCA a U (Ty_Lam b K T) (Ty_Lam c K T')
+  | STCA_TyLam3 : forall b K T T',
+      a <> b ->
+      ~ appears_free_in_Ty b U ->
+      substituteTCA a U T T' ->
+      substituteTCA a U (Ty_Lam b K T) (Ty_Lam b K T')
+  | STCA_TyApp : forall T1 T1' T2 T2',
+      substituteTCA a U T1 T1' ->
+      substituteTCA a U T2 T2' ->
+      substituteTCA a U (Ty_App T1 T2) (Ty_App T1' T2')
+  .
+
+(** * Capture-avoiding multi-substitutions of types *)
+
+Definition env := list (tyname * Ty).
+
+Inductive msubstTCA : env -> Ty -> Ty -> Prop :=
+  | msubstTCA_nil : forall T,
+      msubstTCA nil T T
+  | msubstTCA_cons : forall a U ss T T' T'',
+      substituteTCA a U T T' ->
+      msubstTCA ss T' T'' ->
+      msubstTCA ((a, U) :: ss) T T''.
