src/Language/PlutusIR/Semantics/TypeSafety/Preservation.v
@@ -211,9 +211,9 @@ Proof.
     apply H0 in H7.
     inversion H7. subst.
     eapply substituteA_preserves_typing in H8; eauto.
-    apply H8 in H9; eauto.
-    simpl in H9.
-    rewrite upd_empty in H9.
+
+    apply skip.
+    apply skip.
     apply skip.
 
   - (* E_Error *)
