src/Language/PlutusIR/Semantics/TypeSafety/SubstitutionPreservesTyping/SubstituteTCA.v
@@ -1,0 +1,102 @@
+Require Import PlutusCert.Language.PlutusIR.
+Import NamedTerm.
+Require Import PlutusCert.Language.PlutusIR.Semantics.Static.
+
+
+
+Theorem substituteTCA_preserves_kinding : forall T T' Delta X K U L,
+  (X |-> L; Delta) |-* T : K ->
+  empty |-* U : L ->
+  substituteTCA X U T T' ->
+  Delta |-* T' : K.
+Proof.
+  intros T T' Delta X K U L Hkind Hkind' Hstca__T'.
+  generalize dependent L.
+  generalize dependent U.
+  generalize dependent K.
+  generalize dependent X.
+  generalize dependent Delta.
+  generalize dependent T'.
+
+  induction T.
+  - (* Ty_Var *)
+    intros.
+    rename t into Y.
+    inversion Hkind. subst.
+    inversion Hstca__T'.
+    + (* STCA_TyVar1 *)
+      subst.
+      apply weakening_empty__has_kind.
+      rewrite update_eq in H1.
+      inversion H1.
+      subst.
+      apply Hkind'.
+    + (* STCA_TyVar2 *)
+      subst.
+      rewrite update_neq in H1; auto.
+      auto with typing.
+  - (* Ty_Fun *)
+    intros.
+    inversion Hkind. subst.
+    inversion Hstca__T'. subst.
+    eauto with typing.
+  - (* Ty_IFix *)
+    intros.
+    inversion Hkind. subst.
+    inversion Hstca__T'. subst.
+    simpl.
+    eauto with typing.
+  - (* Ty_Forall *)
+    intros.
+    rename b into bX.
+    inversion Hkind. subst.
+    inversion Hstca__T'. subst.
+    + (* STCA_TyForall1 *)
+      subst.
+      apply K_Forall.
+      rewrite update_shadow in H4.
+      assumption.
+    + (* STCA_TyForall2 *)
+      subst.
+      apply K_Forall.
+      apply skip. (* TODO *)
+    + (* STCA_TyForall3 *)
+      apply K_Forall.
+      eapply IHT; eauto.
+      rewrite update_permute.
+      assumption.
+      auto.
+  - (* Ty_Builtin *)
+    intros.
+    inversion Hkind. subst.
+    inversion Hstca__T'. subst.
+    simpl.
+    apply K_Builtin.
+  - (* Ty_Lam *)  
+    intros.
+    inversion Hkind. subst.
+    rename b into bX.
+    simpl.
+    inversion Hstca__T'.
+    + (* STCA_TyLam1 *)
+      subst.
+      apply K_Lam.
+      rewrite update_shadow in H4.
+      assumption.
+    + (* STCA_TyLam2 *)
+      subst.
+      apply K_Lam.
+      apply skip.
+    + (* STCA_TyLam3 *)
+      subst.
+      apply K_Lam.
+      rewrite update_permute in H4.
+      eauto.
+      assumption.
+  - (* Ty_App *)
+    intros. 
+    inversion Hkind. subst.
+    inversion Hstca__T'. subst.
+    simpl.
+    eauto with typing.
+Qed.
